Working examples.

tests/Add.bpl
@@ -10,10 +10,8 @@ type State;
 var M: MType;
 var C: CType;
 var R: CType;
-var L: CType;
+var I: CType;
 var St: [Actor]State;
-const Base#L: int;
-axiom 1 <= Base#L;
 
 const unique this#: Actor;
 type List a = [int]a;
@@ -21,213 +19,263 @@ var AT#intlst: List int;
 
 function AT#Min(x:int, y: int): int { if x <= y then x else y }
 
-// -- Sequence numbering for FT ----------------------------------
-var SqnCh: <a>[Chan a][int]int;
-var SqnAct: [Actor]int;
-
 // ---------------------------------------------------------------
 // -- End of prelude ---------------------------------------------
 // ---------------------------------------------------------------
 
-procedure Add#anon$0#0()
-  modifies C, R, M, St, SqnCh, SqnAct;
+procedure Add#init#0()
+  modifies C, R, M, I, St;
 {
   var in1: Chan (int);
   var in2: Chan (int);
   var out: Chan (int);
-  assume SqnCh[in1][0] == SqnCh[in2][0];
-  assume true;
-  assume true;
+  assume (in1 != in2) && (in1 != out) && (in2 != out);
+  assume R[in1] == 0;
+  assume R[in2] == 0;
+  assume C[out] == 0;
+  assert {:msg "Initialization might not establish the invariant (#0)"} R[in1] == C[out];
+  assert {:msg "Initialization might not establish the invariant (#1)"} R[in2] == C[out];
+  assert {:msg "Initialization might not establish the invariant (#2)"} (forall idx$: int :: 
+    (0 <= idx$) && (idx$ < C[out]) ==> (M[out][idx$] == (M[in1][idx$] + M[in2][idx$]))
+  );
 }
-procedure Net#init#1()
-  modifies C, R, M, St, SqnCh, SqnAct;
+procedure Add#anon$0#1()
+  modifies C, R, M, I, St;
 {
-  assume C[Net#a] == 0;
-  assume R[Net#a] == 0;
-  assume C[Net#b] == 0;
-  assume R[Net#b] == 0;
-  assume C[Net#c] == 0;
-  assume R[Net#c] == 0;
-}
-const unique Net#add: Actor;
-const unique Net#a: Chan (int);
-const unique Net#b: Chan (int);
-const unique Net#c: Chan (int);
-procedure Net#anon$2#entry#2()
-  modifies C, R, M, St, SqnCh, SqnAct;
-{
-  assume SqnAct[Net#add] == 0;
-  assume L[Net#a] == (1 * Base#L);
-  assume L[Net#b] == (1 * Base#L);
-  assume R[Net#a] == 0;
-  assume C[Net#a] == 0;
-  assume R[Net#b] == 0;
-  assume C[Net#b] == 0;
-  assume R[Net#c] == 0;
-  assume C[Net#c] == 0;
+  var in1: Chan (int);
+  var in2: Chan (int);
+  var out: Chan (int);
+  var in1#0: int;
+  var in2#0: int;
+  assume (in1 != in2) && (in1 != out) && (in2 != out);
+  assume 0 <= R[in1];
+  assume 0 <= R[in2];
+  assume 0 <= C[out];
+  assume R[in1] == C[out];
+  assume R[in2] == C[out];
   assume (forall idx$: int :: 
-    (0 <= idx$) && (idx$ < L[Net#a]) ==> (0 <= M[Net#a][idx$]) && (0 <= M[Net#b][idx$])
+    (0 <= idx$) && (idx$ < C[out]) ==> (M[out][idx$] == (M[in1][idx$] + M[in2][idx$]))
   );
-  assume 0 <= R[Net#a];
-  assume 0 <= C[Net#a];
-  assume (R[Net#a] + C[Net#a]) <= L[Net#a];
-  assume 0 <= R[Net#b];
-  assume 0 <= C[Net#b];
-  assume (R[Net#b] + C[Net#b]) <= L[Net#b];
-  assume 0 <= R[Net#c];
-  assume 0 <= C[Net#c];
-  assume R[Net#c] == 0;
-  assert {:msg "  Channel invariant might not hold on action entry (#9)"} (forall idx$: int :: 
-    (0 <= idx$) && (idx$ < L[Net#a]) ==> (0 <= M[Net#a][idx$]) && (0 <= M[Net#b][idx$])
-  );
-  assert {:msg "  Channel invariant might not hold on action entry (#10)"} R[Net#a] == (R[Net#c] + C[Net#c]);
-  assert {:msg "  Channel invariant might not hold on action entry (#11)"} R[Net#b] == (R[Net#c] + C[Net#c]);
-  assert {:msg "  Channel invariant might not hold on action entry (#12)"} (forall idx$: int :: 
-    (0 <= idx$) && (idx$ < (R[Net#c] + C[Net#c])) ==> (M[Net#c][idx$] == (M[Net#a][idx$] + M[Net#b][idx$]))
-  );
-  assert {:msg "  Channel invariant might not hold on action entry (#13)"} (forall idx$: int :: 
-    (0 <= idx$) && (idx$ < (R[Net#a] + C[Net#a])) ==> (SqnCh[Net#a][idx$] == idx$)
-  );
-  assert {:msg "  Channel invariant might not hold on action entry (#14)"} (forall idx$: int :: 
-    (0 <= idx$) && (idx$ < (R[Net#b] + C[Net#b])) ==> (SqnCh[Net#b][idx$] == idx$)
-  );
-  assert {:msg "  16.3: Channel invariant might not hold on action entry (#15)"} SqnAct[Net#add] == R[Net#a];
-  assert {:msg "  17.3: Channel invariant might not hold on action entry (#16)"} (forall i: int :: 
-    (0 <= i) && (i < (R[Net#a] + C[Net#a])) ==> (SqnCh[Net#a][i] == SqnCh[Net#b][i])
-  );
-  assert {:msg "  18.3: Channel invariant might not hold on action entry (#17)"} (forall i: int :: 
-    (0 <= i) && (i < R[Net#a]) ==> (SqnCh[Net#a][i] == SqnCh[Net#c][i])
+  in1#0 := M[in1][R[in1]];
+  R[in1] := R[in1] + 1;
+  in2#0 := M[in2][R[in2]];
+  R[in2] := R[in2] + 1;
+  assume true;
+  M[out][C[out]] := in1#0 + in2#0;
+  C[out] := C[out] + 1;
+  assert {:msg "Action at 3.3 might not preserve invariant (#3)"} R[in1] == C[out];
+  assert {:msg "Action at 3.3 might not preserve invariant (#4)"} R[in2] == C[out];
+  assert {:msg "Action at 3.3 might not preserve invariant (#5)"} (forall idx$: int :: 
+    (0 <= idx$) && (idx$ < C[out]) ==> (M[out][idx$] == (M[in1][idx$] + M[in2][idx$]))
   );
 }
-procedure Net#anon$2#Add#anon$0#3()
-  modifies C, R, M, St, SqnCh, SqnAct;
+procedure Net#init#2()
+  modifies C, R, M, I, St;
 {
-  var St#next: State;
+  var Net#add: Actor;
+  var Net#a: Chan (int);
+  var Net#b: Chan (int);
+  var Net#c: Chan (int);
+  assume (Net#a != Net#b) && (Net#a != Net#c) && (Net#b != Net#c);
+  assume 0 <= I[Net#a];
+  assume I[Net#a] <= R[Net#a];
+  assume R[Net#a] <= C[Net#a];
+  assume 0 <= I[Net#b];
+  assume I[Net#b] <= R[Net#b];
+  assume R[Net#b] <= C[Net#b];
+  assume 0 <= I[Net#c];
+  assume I[Net#c] <= R[Net#c];
+  assume R[Net#c] <= C[Net#c];
+  assume I[Net#c] == R[Net#c];
+  assume C[Net#a] == 0;
+  assume R[Net#a] == 0;
+  assume C[Net#b] == 0;
+  assume R[Net#b] == 0;
+  assume C[Net#c] == 0;
+  assume R[Net#c] == 0;
+  assume R[Net#a] == C[Net#c];
+  assume R[Net#b] == C[Net#c];
+  assume (forall idx$: int :: 
+    (0 <= idx$) && (idx$ < C[Net#c]) ==> (M[Net#c][idx$] == (M[Net#a][idx$] + M[Net#b][idx$]))
+  );
+  assert {:msg "Initialization of network 'Net' might not establish the channel invariant (#6)"} I[Net#c] == I[Net#a];
+  assert {:msg "Initialization of network 'Net' might not establish the channel invariant (#7)"} I[Net#c] == I[Net#b];
+  I := R;
+  assert {:msg "17.5: The initialization might produce unspecified tokens on channel a (#8)"} (C[Net#a] - R[Net#a]) == 0;
+  assert {:msg "18.5: The initialization might produce unspecified tokens on channel b (#9)"} (C[Net#b] - R[Net#b]) == 0;
+  assert {:msg "19.5: The initialization might produce unspecified tokens on channel c (#10)"} (C[Net#c] - R[Net#c]) == 0;
+}
+procedure Net##Add#anon$0#3()
+  modifies C, R, M, I, St;
+{
+  var Net#add: Actor;
+  var Net#a: Chan (int);
+  var Net#b: Chan (int);
+  var Net#c: Chan (int);
   var in1#i: int;
   var in2#j: int;
-  assume L[Net#a] == (1 * Base#L);
-  assume L[Net#b] == (1 * Base#L);
-  assume 0 <= R[Net#a];
-  assume 0 <= C[Net#a];
-  assume (R[Net#a] + C[Net#a]) <= L[Net#a];
-  assume 0 <= R[Net#b];
-  assume 0 <= C[Net#b];
-  assume (R[Net#b] + C[Net#b]) <= L[Net#b];
-  assume 0 <= R[Net#c];
-  assume 0 <= C[Net#c];
-  assume R[Net#c] == 0;
+  assume (Net#a != Net#b) && (Net#a != Net#c) && (Net#b != Net#c);
+  assume 0 <= I[Net#a];
+  assume I[Net#a] <= R[Net#a];
+  assume R[Net#a] <= C[Net#a];
+  assume 0 <= I[Net#b];
+  assume I[Net#b] <= R[Net#b];
+  assume R[Net#b] <= C[Net#b];
+  assume 0 <= I[Net#c];
+  assume I[Net#c] <= R[Net#c];
+  assume R[Net#c] <= C[Net#c];
+  assume I[Net#c] == R[Net#c];
+  assume I[Net#c] == I[Net#a];
+  assume I[Net#c] == I[Net#b];
+  assume R[Net#a] == C[Net#c];
+  assume R[Net#b] == C[Net#c];
   assume (forall idx$: int :: 
-    (0 <= idx$) && (idx$ < L[Net#a]) ==> (0 <= M[Net#a][idx$]) && (0 <= M[Net#b][idx$])
+    (0 <= idx$) && (idx$ < C[Net#c]) ==> (M[Net#c][idx$] == (M[Net#a][idx$] + M[Net#b][idx$]))
   );
-  assume R[Net#a] == (R[Net#c] + C[Net#c]);
-  assume R[Net#b] == (R[Net#c] + C[Net#c]);
+  assume (1 <= (C[Net#a] - R[Net#a])) && (1 <= (C[Net#b] - R[Net#b]));
+  assume R[Net#a] == C[Net#c];
+  assume R[Net#b] == C[Net#c];
   assume (forall idx$: int :: 
-    (0 <= idx$) && (idx$ < (R[Net#c] + C[Net#c])) ==> (M[Net#c][idx$] == (M[Net#a][idx$] + M[Net#b][idx$]))
+    (0 <= idx$) && (idx$ < C[Net#c]) ==> (M[Net#c][idx$] == (M[Net#a][idx$] + M[Net#b][idx$]))
   );
-  assume (forall idx$: int :: 
-    (0 <= idx$) && (idx$ < (R[Net#a] + C[Net#a])) ==> (SqnCh[Net#a][idx$] == idx$)
-  );
-  assume (forall idx$: int :: 
-    (0 <= idx$) && (idx$ < (R[Net#b] + C[Net#b])) ==> (SqnCh[Net#b][idx$] == idx$)
-  );
-  assume SqnAct[Net#add] == R[Net#a];
-  assume (forall i: int :: 
-    (0 <= i) && (i < (R[Net#a] + C[Net#a])) ==> (SqnCh[Net#a][i] == SqnCh[Net#b][i])
-  );
-  assume (forall i: int :: 
-    (0 <= i) && (i < R[Net#a]) ==> (SqnCh[Net#a][i] == SqnCh[Net#c][i])
-  );
-  assume true;
-  assume (1 <= C[Net#a]) && (1 <= C[Net#b]);
-  assert {:msg "  4.14: Precondition might not hold for instance at 21.5"} SqnCh[Net#a][R[Net#a] - 0] == SqnCh[Net#b][R[Net#b] - 0];
   in1#i := M[Net#a][R[Net#a]];
   R[Net#a] := R[Net#a] + 1;
-  C[Net#a] := C[Net#a] - 1;
   in2#j := M[Net#b][R[Net#b]];
   R[Net#b] := R[Net#b] + 1;
-  C[Net#b] := C[Net#b] - 1;
-  M[Net#c][R[Net#c] + C[Net#c]] := in1#i + in2#j;
-  SqnCh[Net#c][R[Net#c] + C[Net#c]] := SqnAct[Net#add];
+  M[Net#c][C[Net#c]] := in1#i + in2#j;
   C[Net#c] := C[Net#c] + 1;
-  SqnAct[Net#add] := SqnAct[Net#add] + 1;
-  assume 0 <= R[Net#a];
-  assume 0 <= C[Net#a];
-  assume (R[Net#a] + C[Net#a]) <= L[Net#a];
-  assume 0 <= R[Net#b];
-  assume 0 <= C[Net#b];
-  assume (R[Net#b] + C[Net#b]) <= L[Net#b];
-  assume 0 <= R[Net#c];
-  assume 0 <= C[Net#c];
-  assume R[Net#c] == 0;
-  assert {:msg "  Action at 3.3 ('anon$0') for actor instance 'add' might not preserve the channel invariant (#27)"} (forall idx$: int :: 
-    (0 <= idx$) && (idx$ < L[Net#a]) ==> (0 <= M[Net#a][idx$]) && (0 <= M[Net#b][idx$])
+  assume R[Net#a] == C[Net#c];
+  assume R[Net#b] == C[Net#c];
+  assume (forall idx$: int :: 
+    (0 <= idx$) && (idx$ < C[Net#c]) ==> (M[Net#c][idx$] == (M[Net#a][idx$] + M[Net#b][idx$]))
   );
-  assert {:msg "  Action at 3.3 ('anon$0') for actor instance 'add' might not preserve the channel invariant (#28)"} R[Net#a] == (R[Net#c] + C[Net#c]);
-  assert {:msg "  Action at 3.3 ('anon$0') for actor instance 'add' might not preserve the channel invariant (#29)"} R[Net#b] == (R[Net#c] + C[Net#c]);
-  assert {:msg "  Action at 3.3 ('anon$0') for actor instance 'add' might not preserve the channel invariant (#30)"} (forall idx$: int :: 
-    (0 <= idx$) && (idx$ < (R[Net#c] + C[Net#c])) ==> (M[Net#c][idx$] == (M[Net#a][idx$] + M[Net#b][idx$]))
-  );
-  assert {:msg "  Action at 3.3 ('anon$0') for actor instance 'add' might not preserve the channel invariant (#31)"} (forall idx$: int :: 
-    (0 <= idx$) && (idx$ < (R[Net#a] + C[Net#a])) ==> (SqnCh[Net#a][idx$] == idx$)
-  );
-  assert {:msg "  Action at 3.3 ('anon$0') for actor instance 'add' might not preserve the channel invariant (#32)"} (forall idx$: int :: 
-    (0 <= idx$) && (idx$ < (R[Net#b] + C[Net#b])) ==> (SqnCh[Net#b][idx$] == idx$)
-  );
-  assert {:msg "  16.3: Action at 3.3 ('anon$0') for actor instance 'add' might not preserve the channel invariant (#33)"} SqnAct[Net#add] == R[Net#a];
-  assert {:msg "  17.3: Action at 3.3 ('anon$0') for actor instance 'add' might not preserve the channel invariant (#34)"} (forall i: int :: 
-    (0 <= i) && (i < (R[Net#a] + C[Net#a])) ==> (SqnCh[Net#a][i] == SqnCh[Net#b][i])
-  );
-  assert {:msg "  18.3: Action at 3.3 ('anon$0') for actor instance 'add' might not preserve the channel invariant (#35)"} (forall i: int :: 
-    (0 <= i) && (i < R[Net#a]) ==> (SqnCh[Net#a][i] == SqnCh[Net#c][i])
-  );
+  assert {:msg "Action at 3.3 ('anon$0') for actor instance 'add' might not preserve the channel invariant (#11)"} I[Net#c] == I[Net#a];
+  assert {:msg "Action at 3.3 ('anon$0') for actor instance 'add' might not preserve the channel invariant (#12)"} I[Net#c] == I[Net#b];
 }
-procedure Net#anon$2#exit#4()
-  modifies C, R, M, St, SqnCh, SqnAct;
+procedure Net#entry()
+  modifies C, R, M, I, St;
 {
-  assume L[Net#a] == (1 * Base#L);
-  assume L[Net#b] == (1 * Base#L);
-  assume 0 <= R[Net#a];
-  assume 0 <= C[Net#a];
-  assume (R[Net#a] + C[Net#a]) <= L[Net#a];
-  assume 0 <= R[Net#b];
-  assume 0 <= C[Net#b];
-  assume (R[Net#b] + C[Net#b]) <= L[Net#b];
-  assume 0 <= R[Net#c];
-  assume 0 <= C[Net#c];
-  assume R[Net#c] == 0;
+  var Net#add: Actor;
+  var Net#a: Chan (int);
+  var Net#b: Chan (int);
+  var Net#c: Chan (int);
+  assume (Net#a != Net#b) && (Net#a != Net#c) && (Net#b != Net#c);
+  assume 0 <= I[Net#a];
+  assume I[Net#a] <= R[Net#a];
+  assume R[Net#a] <= C[Net#a];
+  assume 0 <= I[Net#b];
+  assume I[Net#b] <= R[Net#b];
+  assume R[Net#b] <= C[Net#b];
+  assume 0 <= I[Net#c];
+  assume I[Net#c] <= R[Net#c];
+  assume R[Net#c] <= C[Net#c];
+  assume I[Net#c] == R[Net#c];
+  assume C[Net#a] == R[Net#a];
+  assume C[Net#b] == R[Net#b];
+  assume C[Net#c] == R[Net#c];
+  assume I[Net#c] == I[Net#a];
+  assume I[Net#c] == I[Net#b];
+  assume R[Net#a] == C[Net#c];
+  assume R[Net#b] == C[Net#c];
   assume (forall idx$: int :: 
-    (0 <= idx$) && (idx$ < L[Net#a]) ==> (0 <= M[Net#a][idx$]) && (0 <= M[Net#b][idx$])
+    (0 <= idx$) && (idx$ < C[Net#c]) ==> (M[Net#c][idx$] == (M[Net#a][idx$] + M[Net#b][idx$]))
   );
-  assume R[Net#a] == (R[Net#c] + C[Net#c]);
-  assume R[Net#b] == (R[Net#c] + C[Net#c]);
+  assert {:msg "6.1: Sub-actors in the network might fire without network input. This is not permitted. (#13)"} !((1 <= (C[Net#a] - R[Net#a])) && (1 <= (C[Net#b] - R[Net#b])));
+}
+procedure Net#anon$1#input#in1#4()
+  modifies C, R, M, I, St;
+{
+  var Net#add: Actor;
+  var Net#a: Chan (int);
+  var Net#b: Chan (int);
+  var Net#c: Chan (int);
+  assume (Net#a != Net#b) && (Net#a != Net#c) && (Net#b != Net#c);
+  assume 0 <= I[Net#a];
+  assume I[Net#a] <= R[Net#a];
+  assume R[Net#a] <= C[Net#a];
+  assume 0 <= I[Net#b];
+  assume I[Net#b] <= R[Net#b];
+  assume R[Net#b] <= C[Net#b];
+  assume 0 <= I[Net#c];
+  assume I[Net#c] <= R[Net#c];
+  assume R[Net#c] <= C[Net#c];
+  assume I[Net#c] == R[Net#c];
+  assume C[Net#a] < 1;
+  assume I[Net#c] == I[Net#a];
+  assume I[Net#c] == I[Net#b];
+  assume R[Net#a] == C[Net#c];
+  assume R[Net#b] == C[Net#c];
   assume (forall idx$: int :: 
-    (0 <= idx$) && (idx$ < (R[Net#c] + C[Net#c])) ==> (M[Net#c][idx$] == (M[Net#a][idx$] + M[Net#b][idx$]))
+    (0 <= idx$) && (idx$ < C[Net#c]) ==> (M[Net#c][idx$] == (M[Net#a][idx$] + M[Net#b][idx$]))
   );
+  C[Net#a] := C[Net#a] + 1;
+  assert {:msg "Channel invariant might be falsified by network input (#14)"} I[Net#c] == I[Net#a];
+  assert {:msg "Channel invariant might be falsified by network input (#15)"} I[Net#c] == I[Net#b];
+}
+procedure Net#anon$1#input#in2#5()
+  modifies C, R, M, I, St;
+{
+  var Net#add: Actor;
+  var Net#a: Chan (int);
+  var Net#b: Chan (int);
+  var Net#c: Chan (int);
+  assume (Net#a != Net#b) && (Net#a != Net#c) && (Net#b != Net#c);
+  assume 0 <= I[Net#a];
+  assume I[Net#a] <= R[Net#a];
+  assume R[Net#a] <= C[Net#a];
+  assume 0 <= I[Net#b];
+  assume I[Net#b] <= R[Net#b];
+  assume R[Net#b] <= C[Net#b];
+  assume 0 <= I[Net#c];
+  assume I[Net#c] <= R[Net#c];
+  assume R[Net#c] <= C[Net#c];
+  assume I[Net#c] == R[Net#c];
+  assume C[Net#b] < 1;
+  assume I[Net#c] == I[Net#a];
+  assume I[Net#c] == I[Net#b];
+  assume R[Net#a] == C[Net#c];
+  assume R[Net#b] == C[Net#c];
   assume (forall idx$: int :: 
-    (0 <= idx$) && (idx$ < (R[Net#a] + C[Net#a])) ==> (SqnCh[Net#a][idx$] == idx$)
+    (0 <= idx$) && (idx$ < C[Net#c]) ==> (M[Net#c][idx$] == (M[Net#a][idx$] + M[Net#b][idx$]))
   );
+  C[Net#b] := C[Net#b] + 1;
+  assert {:msg "Channel invariant might be falsified by network input (#16)"} I[Net#c] == I[Net#a];
+  assert {:msg "Channel invariant might be falsified by network input (#17)"} I[Net#c] == I[Net#b];
+}
+procedure Net#anon$1#exit#6()
+  modifies C, R, M, I, St;
+{
+  var Net#add: Actor;
+  var Net#a: Chan (int);
+  var Net#b: Chan (int);
+  var Net#c: Chan (int);
+  assume (Net#a != Net#b) && (Net#a != Net#c) && (Net#b != Net#c);
+  assume 0 <= I[Net#a];
+  assume I[Net#a] <= R[Net#a];
+  assume R[Net#a] <= C[Net#a];
+  assume 0 <= I[Net#b];
+  assume I[Net#b] <= R[Net#b];
+  assume R[Net#b] <= C[Net#b];
+  assume 0 <= I[Net#c];
+  assume I[Net#c] <= R[Net#c];
+  assume R[Net#c] <= C[Net#c];
+  assume I[Net#c] == R[Net#c];
+  assume I[Net#c] == I[Net#a];
+  assume I[Net#c] == I[Net#b];
+  assume R[Net#a] == C[Net#c];
+  assume R[Net#b] == C[Net#c];
   assume (forall idx$: int :: 
-    (0 <= idx$) && (idx$ < (R[Net#b] + C[Net#b])) ==> (SqnCh[Net#b][idx$] == idx$)
+    (0 <= idx$) && (idx$ < C[Net#c]) ==> (M[Net#c][idx$] == (M[Net#a][idx$] + M[Net#b][idx$]))
   );
-  assume SqnAct[Net#add] == R[Net#a];
-  assume (forall i: int :: 
-    (0 <= i) && (i < (R[Net#a] + C[Net#a])) ==> (SqnCh[Net#a][i] == SqnCh[Net#b][i])
-  );
-  assume (forall i: int :: 
-    (0 <= i) && (i < R[Net#a]) ==> (SqnCh[Net#a][i] == SqnCh[Net#c][i])
-  );
-  assume !((R[Net#a] + C[Net#a]) < L[Net#a]);
-  assume !((R[Net#b] + C[Net#b]) < L[Net#b]);
-  assume !((1 <= C[Net#a]) && (1 <= C[Net#b]));
-  assert {:msg "  12.13: Network action postcondition might not hold"} (forall idx$: int :: 
-    (0 <= idx$) && (idx$ < L[Net#a]) ==> (M[Net#c][0] == (M[Net#a][idx$] + M[Net#b][idx$]))
-  );
-  assert {:msg "  13.13: Network action postcondition might not hold"} (forall idx$: int :: 
-    (0 <= idx$) && (idx$ < L[Net#a]) ==> (SqnCh[Net#c][0] == 0)
-  );
-  R[Net#c] := R[Net#c] + C[Net#c];
-  C[Net#c] := C[Net#c] - (1 * Base#L);
-  assert {:msg "  The network might leave unread tokens on channel a"} C[Net#a] == 0;
-  assert {:msg "  The network might leave unread tokens on channel b"} C[Net#b] == 0;
-  assert {:msg "  The network might not produce the specified number of tokens on output out"} C[Net#c] == 0;
+  assume (C[Net#a] - I[Net#a]) == 1;
+  assume (C[Net#b] - I[Net#b]) == 1;
+  assume !((1 <= (C[Net#a] - R[Net#a])) && (1 <= (C[Net#b] - R[Net#b])));
+  assert {:msg "9.13: Network action postcondition might not hold (#18)"} M[Net#c][I[Net#c]] == (M[Net#a][I[Net#a]] + M[Net#b][I[Net#b]]);
+  R[Net#c] := R[Net#c] + 1;
+  I := R;
+  assert {:msg "The network might not preserve the channel invariant (#19)"} I[Net#c] == I[Net#a];
+  assert {:msg "The network might not preserve the channel invariant (#20)"} I[Net#c] == I[Net#b];
+  assert {:msg "8.3: The network might leave unread tokens on channel a (#21)"} C[Net#a] == R[Net#a];
+  assert {:msg "8.3: The network might leave unread tokens on channel b (#22)"} C[Net#b] == R[Net#b];
+  assert {:msg "8.3: The network might not produce the specified number of tokens on output out (#23)"} C[Net#c] == R[Net#c];
 }
