tests/AddDelay.bpl
@@ -10,12 +10,8 @@ type State;
 var M: MType;
 var C: CType;
 var R: CType;
-var L: CType;
 var I: CType;
 var St: [Actor]State;
-
-const Base#L: int;
-axiom 1 <= Base#L;
 
 const unique this#: Actor;
 type List a = [int]a;
@@ -27,35 +23,163 @@ function AT#Min(x:int, y: int): int { if x <= y then x else y }
 // -- End of prelude ---------------------------------------------
 // ---------------------------------------------------------------
 
-procedure Add#anon$0#0()
+procedure Add#init#0()
   modifies C, R, M, I, St;
 {
   var in1: Chan (int);
   var in2: Chan (int);
   var out: Chan (int);
-  assume true;
-  assume true;
+  assume (in1 != in2) && (in1 != out) && (in2 != out);
+  assume R[in1] == 0;
+  assume R[in2] == 0;
+  assume C[out] == 0;
+  assert {:msg "Initialization might not establish the invariant (#0)"} R[in1] == C[out];
+  assert {:msg "Initialization might not establish the invariant (#1)"} R[in2] == C[out];
+  assert {:msg "Initialization might not establish the invariant (#2)"} (forall idx$: int :: 
+    (0 <= idx$) && (idx$ < C[out]) ==> (M[out][idx$] == (M[in1][idx$] + M[in2][idx$]))
+  );
 }
-procedure Delay#anon$1#1()
+procedure Add#anon$0#1()
+  modifies C, R, M, I, St;
+{
+  var in1: Chan (int);
+  var in2: Chan (int);
+  var out: Chan (int);
+  var in1#0: int;
+  var in2#0: int;
+  assume (in1 != in2) && (in1 != out) && (in2 != out);
+  assume 0 <= R[in1];
+  assume 0 <= R[in2];
+  assume 0 <= C[out];
+  assume R[in1] == C[out];
+  assume R[in2] == C[out];
+  assume (forall idx$: int :: 
+    (0 <= idx$) && (idx$ < C[out]) ==> (M[out][idx$] == (M[in1][idx$] + M[in2][idx$]))
+  );
+  in1#0 := M[in1][R[in1]];
+  R[in1] := R[in1] + 1;
+  in2#0 := M[in2][R[in2]];
+  R[in2] := R[in2] + 1;
+  assume true;
+  M[out][C[out]] := in1#0 + in2#0;
+  C[out] := C[out] + 1;
+  assert {:msg "Action at 2.3 might not preserve invariant (#3)"} R[in1] == C[out];
+  assert {:msg "Action at 2.3 might not preserve invariant (#4)"} R[in2] == C[out];
+  assert {:msg "Action at 2.3 might not preserve invariant (#5)"} (forall idx$: int :: 
+    (0 <= idx$) && (idx$ < C[out]) ==> (M[out][idx$] == (M[in1][idx$] + M[in2][idx$]))
+  );
+}
+procedure Split#init#2()
+  modifies C, R, M, I, St;
+{
+  var in: Chan (int);
+  var out1: Chan (int);
+  var out2: Chan (int);
+  assume (in != out1) && (in != out2) && (out1 != out2);
+  assume R[in] == 0;
+  assume C[out1] == 0;
+  assume C[out2] == 0;
+  assert {:msg "Initialization might not establish the invariant (#6)"} R[in] == C[out1];
+  assert {:msg "Initialization might not establish the invariant (#7)"} R[in] == C[out2];
+  assert {:msg "Initialization might not establish the invariant (#8)"} (forall idx$: int :: 
+    (0 <= idx$) && (idx$ < C[out1]) ==> (M[out1][idx$] == M[in][idx$])
+  );
+  assert {:msg "Initialization might not establish the invariant (#9)"} (forall idx$: int :: 
+    (0 <= idx$) && (idx$ < C[out2]) ==> (M[out2][idx$] == M[in][idx$])
+  );
+}
+procedure Split#anon$1#3()
+  modifies C, R, M, I, St;
+{
+  var in: Chan (int);
+  var out1: Chan (int);
+  var out2: Chan (int);
+  var in#0: int;
+  assume (in != out1) && (in != out2) && (out1 != out2);
+  assume 0 <= R[in];
+  assume 0 <= C[out1];
+  assume 0 <= C[out2];
+  assume R[in] == C[out1];
+  assume R[in] == C[out2];
+  assume (forall idx$: int :: 
+    (0 <= idx$) && (idx$ < C[out1]) ==> (M[out1][idx$] == M[in][idx$])
+  );
+  assume (forall idx$: int :: 
+    (0 <= idx$) && (idx$ < C[out2]) ==> (M[out2][idx$] == M[in][idx$])
+  );
+  in#0 := M[in][R[in]];
+  R[in] := R[in] + 1;
+  assume true;
+  M[out1][C[out1]] := in#0;
+  C[out1] := C[out1] + 1;
+  M[out2][C[out2]] := in#0;
+  C[out2] := C[out2] + 1;
+  assert {:msg "Action at 6.3 might not preserve invariant (#10)"} R[in] == C[out1];
+  assert {:msg "Action at 6.3 might not preserve invariant (#11)"} R[in] == C[out2];
+  assert {:msg "Action at 6.3 might not preserve invariant (#12)"} (forall idx$: int :: 
+    (0 <= idx$) && (idx$ < C[out1]) ==> (M[out1][idx$] == M[in][idx$])
+  );
+  assert {:msg "Action at 6.3 might not preserve invariant (#13)"} (forall idx$: int :: 
+    (0 <= idx$) && (idx$ < C[out2]) ==> (M[out2][idx$] == M[in][idx$])
+  );
+}
+procedure Delay#init#4()
   modifies C, R, M, I, St;
 {
   var in: Chan (int);
   var out: Chan (int);
+  var k: int;
+  assume in != out;
+  assume R[in] == 0;
+  assume C[out] == 0;
   assume true;
-  assume true;
+  M[out][C[out]] := k;
+  C[out] := C[out] + 1;
+  assert {:msg "10.20: Initialization might not establish the invariant (#14)"} M[out][0] == k;
+  assert {:msg "Initialization might not establish the invariant (#15)"} R[in] == (C[out] - 1);
+  assert {:msg "Initialization might not establish the invariant (#16)"} (forall idx$: int :: 
+    (1 <= idx$) && (idx$ < C[out]) ==> (M[out][idx$] == M[in][idx$ - 1])
+  );
 }
-procedure Delay#anon$2#2()
+procedure Delay#anon$3#5()
   modifies C, R, M, I, St;
 {
   var in: Chan (int);
   var out: Chan (int);
+  var k: int;
+  var in#0: int;
+  assume in != out;
+  assume 0 <= R[in];
+  assume 0 <= C[out];
+  assume M[out][0] == k;
+  assume R[in] == (C[out] - 1);
+  assume (forall idx$: int :: 
+    (1 <= idx$) && (idx$ < C[out]) ==> (M[out][idx$] == M[in][idx$ - 1])
+  );
+  in#0 := M[in][R[in]];
+  R[in] := R[in] + 1;
   assume true;
-  assume true;
+  M[out][C[out]] := in#0;
+  C[out] := C[out] + 1;
+  assert {:msg "10.20: Action at 12.3 might not preserve invariant (#17)"} M[out][0] == k;
+  assert {:msg "Action at 12.3 might not preserve invariant (#18)"} R[in] == (C[out] - 1);
+  assert {:msg "Action at 12.3 might not preserve invariant (#19)"} (forall idx$: int :: 
+    (1 <= idx$) && (idx$ < C[out]) ==> (M[out][idx$] == M[in][idx$ - 1])
+  );
 }
-procedure Net#init#3()
+procedure Net#init#6()
   modifies C, R, M, I, St;
 {
-  var ActorParam#del#k: int;
+  var Net#add: Actor;
+  var Net#del: Actor;
+  var Net#spl: Actor;
+  var Net#a: Chan (int);
+  var Net#b: Chan (int);
+  var Net#c: Chan (int);
+  var Net#d: Chan (int);
+  var Net#e: Chan (int);
+  assume (Net#add != Net#del) && (Net#add != Net#spl) && (Net#del != Net#spl);
+  assume (Net#a != Net#b) && (Net#a != Net#c) && (Net#a != Net#d) && (Net#a != Net#e) && (Net#b != Net#c) && (Net#b != Net#d) && (Net#b != Net#e) && (Net#c != Net#d) && (Net#c != Net#e) && (Net#d != Net#e);
   assume 0 <= I[Net#a];
   assume I[Net#a] <= R[Net#a];
   assume R[Net#a] <= C[Net#a];
@@ -65,10 +189,13 @@ procedure Net#init#3()
   assume 0 <= I[Net#c];
   assume I[Net#c] <= R[Net#c];
   assume R[Net#c] <= C[Net#c];
-  assume I[Net#c] == R[Net#c];
   assume 0 <= I[Net#d];
   assume I[Net#d] <= R[Net#d];
   assume R[Net#d] <= C[Net#d];
+  assume I[Net#d] == R[Net#d];
+  assume 0 <= I[Net#e];
+  assume I[Net#e] <= R[Net#e];
+  assume R[Net#e] <= C[Net#e];
   assume C[Net#a] == 0;
   assume R[Net#a] == 0;
   assume C[Net#b] == 0;
@@ -77,108 +204,62 @@ procedure Net#init#3()
   assume R[Net#c] == 0;
   assume C[Net#d] == 0;
   assume R[Net#d] == 0;
-  assume ActorParam#del#k == 0;
-  M[Net#b][C[Net#b]] := ActorParam#del#k;
-  C[Net#b] := C[Net#b] + 1;
-  assert {:msg "  Network initialization might not establish the channel invariant (#0)"} (forall i: int :: 
-    (0 <= i) && (i < C[Net#a]) ==> (0 < M[Net#a][i])
-  );
-  assert {:msg "  Network initialization might not establish the channel invariant (#1)"} R[Net#a] == C[Net#c];
-  assert {:msg "  Network initialization might not establish the channel invariant (#2)"} R[Net#b] == C[Net#c];
-  assert {:msg "  Network initialization might not establish the channel invariant (#3)"} R[Net#a] == C[Net#d];
-  assert {:msg "  Network initialization might not establish the channel invariant (#4)"} R[Net#b] == C[Net#d];
-  assert {:msg "  Network initialization might not establish the channel invariant (#5)"} R[Net#d] == (C[Net#b] - 1);
-  assert {:msg "  Network initialization might not establish the channel invariant (#6)"} (forall idx$: int :: 
-    (0 <= idx$) && (idx$ < C[Net#c]) ==> (M[Net#c][idx$] == (M[Net#a][idx$] + M[Net#b][idx$]))
-  );
-  assert {:msg "  Network initialization might not establish the channel invariant (#7)"} (forall idx$: int :: 
-    (0 <= idx$) && (idx$ < C[Net#d]) ==> (M[Net#d][idx$] == (M[Net#a][idx$] + M[Net#b][idx$]))
-  );
-  assert {:msg "  Network initialization might not establish the channel invariant (#8)"} (forall idx$: int :: 
-    (1 <= idx$) && (idx$ < C[Net#b]) ==> (M[Net#b][idx$] == M[Net#d][idx$ - 1])
-  );
-  assert {:msg "  22.15: Network initialization might not establish the channel invariant (#9)"} I[Net#a] == I[Net#c];
-  assert {:msg "  23.15: Network initialization might not establish the channel invariant (#10)"} M[Net#b][0] == 0;
-  C[Net#b] := C[Net#b] - 1;
-}
-const unique Net#add: Actor;
-const unique Net#del: Actor;
-const unique Net#a: Chan (int);
-const unique Net#b: Chan (int);
-const unique Net#c: Chan (int);
-const unique Net#d: Chan (int);
-procedure Net#anon$3#entry#4()
-  modifies C, R, M, I, St;
-{
-  assume 0 <= I[Net#a];
-  assume I[Net#a] <= R[Net#a];
-  assume R[Net#a] <= C[Net#a];
-  assume 0 <= I[Net#b];
-  assume I[Net#b] <= R[Net#b];
-  assume R[Net#b] <= C[Net#b];
-  assume 0 <= I[Net#c];
-  assume I[Net#c] <= R[Net#c];
-  assume R[Net#c] <= C[Net#c];
-  assume I[Net#c] == R[Net#c];
-  assume 0 <= I[Net#d];
-  assume I[Net#d] <= R[Net#d];
-  assume R[Net#d] <= C[Net#d];
-  assume L[Net#a] == (1 * Base#L);
-  assume (R[Net#a] - I[Net#a]) <= L[Net#a];
-  assume (C[Net#a] - R[Net#a]) == 0;
-  assume (C[Net#b] - R[Net#b]) == 0;
-  assume (C[Net#c] - R[Net#c]) == 0;
-  assume (C[Net#d] - R[Net#d]) == 0;
-  assume I == R;
-  C[Net#b] := C[Net#b] + 1;
-  assume (forall i: int :: 
-    (0 <= i) && (i < C[Net#a]) ==> (0 < M[Net#a][i])
-  );
+  assume C[Net#e] == 0;
+  assume R[Net#e] == 0;
   assume R[Net#a] == C[Net#c];
   assume R[Net#b] == C[Net#c];
-  assume R[Net#a] == C[Net#d];
-  assume R[Net#b] == C[Net#d];
-  assume R[Net#d] == (C[Net#b] - 1);
   assume (forall idx$: int :: 
     (0 <= idx$) && (idx$ < C[Net#c]) ==> (M[Net#c][idx$] == (M[Net#a][idx$] + M[Net#b][idx$]))
   );
-  assume (forall idx$: int :: 
-    (0 <= idx$) && (idx$ < C[Net#d]) ==> (M[Net#d][idx$] == (M[Net#a][idx$] + M[Net#b][idx$]))
-  );
-  assume (forall idx$: int :: 
-    (1 <= idx$) && (idx$ < C[Net#b]) ==> (M[Net#b][idx$] == M[Net#d][idx$ - 1])
-  );
-  assume I[Net#a] == I[Net#c];
+  assume 0 == 0;
+  M[Net#b][C[Net#b]] := 0;
+  C[Net#b] := C[Net#b] + 1;
   assume M[Net#b][0] == 0;
-  assume (forall i: int :: 
-    (0 <= i) && (i < C[Net#a]) ==> (0 < M[Net#a][i])
+  assume R[Net#e] == (C[Net#b] - 1);
+  assume (forall idx$: int :: 
+    (1 <= idx$) && (idx$ < C[Net#b]) ==> (M[Net#b][idx$] == M[Net#e][idx$ - 1])
   );
-  assert {:msg "  Channel invariant might not hold on action entry (#11)"} (forall i: int :: 
-    (0 <= i) && (i < C[Net#a]) ==> (0 < M[Net#a][i])
+  assume R[Net#c] == C[Net#d];
+  assume R[Net#c] == C[Net#e];
+  assume (forall idx$: int :: 
+    (0 <= idx$) && (idx$ < C[Net#d]) ==> (M[Net#d][idx$] == M[Net#c][idx$])
   );
-  assert {:msg "  Channel invariant might not hold on action entry (#12)"} R[Net#a] == C[Net#c];
-  assert {:msg "  Channel invariant might not hold on action entry (#13)"} R[Net#b] == C[Net#c];
-  assert {:msg "  Channel invariant might not hold on action entry (#14)"} R[Net#a] == C[Net#d];
-  assert {:msg "  Channel invariant might not hold on action entry (#15)"} R[Net#b] == C[Net#d];
-  assert {:msg "  Channel invariant might not hold on action entry (#16)"} R[Net#d] == (C[Net#b] - 1);
-  assert {:msg "  Channel invariant might not hold on action entry (#17)"} (forall idx$: int :: 
-    (0 <= idx$) && (idx$ < C[Net#c]) ==> (M[Net#c][idx$] == (M[Net#a][idx$] + M[Net#b][idx$]))
+  assume (forall idx$: int :: 
+    (0 <= idx$) && (idx$ < C[Net#e]) ==> (M[Net#e][idx$] == M[Net#c][idx$])
   );
-  assert {:msg "  Channel invariant might not hold on action entry (#18)"} (forall idx$: int :: 
-    (0 <= idx$) && (idx$ < C[Net#d]) ==> (M[Net#d][idx$] == (M[Net#a][idx$] + M[Net#b][idx$]))
+  assert {:msg "25.15: Initialization of network 'Net' might not establish the channel invariant (#20)"} (0 < I[Net#d]) ==> (M[Net#d][0] == M[Net#a][0]);
+  assert {:msg "26.15: Initialization of network 'Net' might not establish the channel invariant (#21)"} (0 < I[Net#d]) ==> (M[Net#d][I[Net#d] - 1] == M[Net#b][I[Net#b]]);
+  assert {:msg "Initialization of network 'Net' might not establish the channel invariant (#22)"} I[Net#c] == I[Net#a];
+  assert {:msg "Initialization of network 'Net' might not establish the channel invariant (#23)"} I[Net#c] == I[Net#b];
+  assert {:msg "Initialization of network 'Net' might not establish the channel invariant (#24)"} I[Net#b] == I[Net#e];
+  assert {:msg "Initialization of network 'Net' might not establish the channel invariant (#25)"} I[Net#d] == I[Net#c];
+  assert {:msg "Initialization of network 'Net' might not establish the channel invariant (#26)"} I[Net#e] == I[Net#c];
+  assert {:msg "Initialization of network 'Net' might not establish the channel invariant (#27)"} true && (forall idx$: int :: 
+    (I[Net#a] <= idx$) && (idx$ < C[Net#a]) ==> (0 <= M[Net#a][idx$])
   );
-  assert {:msg "  Channel invariant might not hold on action entry (#19)"} (forall idx$: int :: 
-    (1 <= idx$) && (idx$ < C[Net#b]) ==> (M[Net#b][idx$] == M[Net#d][idx$ - 1])
-  );
-  assert {:msg "  22.15: Channel invariant might not hold on action entry (#20)"} I[Net#a] == I[Net#c];
-  assert {:msg "  23.15: Channel invariant might not hold on action entry (#21)"} M[Net#b][0] == 0;
+  I := R;
+  C[Net#b] := C[Net#b] - 1;
+  assert {:msg "35.5: The initialization might produce unspecified tokens on channel a (#28)"} (C[Net#a] - R[Net#a]) == 0;
+  assert {:msg "36.5: The initialization might produce unspecified tokens on channel b (#29)"} (C[Net#b] - R[Net#b]) == 0;
+  assert {:msg "37.5: The initialization might produce unspecified tokens on channel c (#30)"} (C[Net#c] - R[Net#c]) == 0;
+  assert {:msg "38.5: The initialization might produce unspecified tokens on channel d (#31)"} (C[Net#d] - R[Net#d]) == 0;
+  assert {:msg "39.5: The initialization might produce unspecified tokens on channel e (#32)"} (C[Net#e] - R[Net#e]) == 0;
 }
-procedure Net#anon$3#Add#anon$0#5()
+procedure Net##Add#anon$0#7()
   modifies C, R, M, I, St;
 {
-  var St#next: State;
+  var Net#add: Actor;
+  var Net#del: Actor;
+  var Net#spl: Actor;
+  var Net#a: Chan (int);
+  var Net#b: Chan (int);
+  var Net#c: Chan (int);
+  var Net#d: Chan (int);
+  var Net#e: Chan (int);
   var in1#i: int;
   var in2#j: int;
+  assume (Net#add != Net#del) && (Net#add != Net#spl) && (Net#del != Net#spl);
+  assume (Net#a != Net#b) && (Net#a != Net#c) && (Net#a != Net#d) && (Net#a != Net#e) && (Net#b != Net#c) && (Net#b != Net#d) && (Net#b != Net#e) && (Net#c != Net#d) && (Net#c != Net#e) && (Net#d != Net#e);
   assume 0 <= I[Net#a];
   assume I[Net#a] <= R[Net#a];
   assume R[Net#a] <= C[Net#a];
@@ -188,67 +269,83 @@ procedure Net#anon$3#Add#anon$0#5()
   assume 0 <= I[Net#c];
   assume I[Net#c] <= R[Net#c];
   assume R[Net#c] <= C[Net#c];
-  assume I[Net#c] == R[Net#c];
   assume 0 <= I[Net#d];
   assume I[Net#d] <= R[Net#d];
   assume R[Net#d] <= C[Net#d];
-  assume L[Net#a] == (1 * Base#L);
-  assume (R[Net#a] - I[Net#a]) <= L[Net#a];
-  assume (forall i: int :: 
-    (0 <= i) && (i < C[Net#a]) ==> (0 < M[Net#a][i])
+  assume I[Net#d] == R[Net#d];
+  assume 0 <= I[Net#e];
+  assume I[Net#e] <= R[Net#e];
+  assume R[Net#e] <= C[Net#e];
+  assume (0 < I[Net#d]) ==> (M[Net#d][0] == M[Net#a][0]);
+  assume (0 < I[Net#d]) ==> (M[Net#d][I[Net#d] - 1] == M[Net#b][I[Net#b]]);
+  assume I[Net#c] == I[Net#a];
+  assume I[Net#c] == I[Net#b];
+  assume I[Net#b] == I[Net#e];
+  assume I[Net#d] == I[Net#c];
+  assume I[Net#e] == I[Net#c];
+  assume true && (forall idx$: int :: 
+    (I[Net#a] <= idx$) && (idx$ < C[Net#a]) ==> (0 <= M[Net#a][idx$])
   );
   assume R[Net#a] == C[Net#c];
   assume R[Net#b] == C[Net#c];
-  assume R[Net#a] == C[Net#d];
-  assume R[Net#b] == C[Net#d];
-  assume R[Net#d] == (C[Net#b] - 1);
   assume (forall idx$: int :: 
     (0 <= idx$) && (idx$ < C[Net#c]) ==> (M[Net#c][idx$] == (M[Net#a][idx$] + M[Net#b][idx$]))
   );
-  assume (forall idx$: int :: 
-    (0 <= idx$) && (idx$ < C[Net#d]) ==> (M[Net#d][idx$] == (M[Net#a][idx$] + M[Net#b][idx$]))
-  );
-  assume (forall idx$: int :: 
-    (1 <= idx$) && (idx$ < C[Net#b]) ==> (M[Net#b][idx$] == M[Net#d][idx$ - 1])
-  );
-  assume I[Net#a] == I[Net#c];
   assume M[Net#b][0] == 0;
-  assume true;
+  assume R[Net#e] == (C[Net#b] - 1);
+  assume (forall idx$: int :: 
+    (1 <= idx$) && (idx$ < C[Net#b]) ==> (M[Net#b][idx$] == M[Net#e][idx$ - 1])
+  );
+  assume R[Net#c] == C[Net#d];
+  assume R[Net#c] == C[Net#e];
+  assume (forall idx$: int :: 
+    (0 <= idx$) && (idx$ < C[Net#d]) ==> (M[Net#d][idx$] == M[Net#c][idx$])
+  );
+  assume (forall idx$: int :: 
+    (0 <= idx$) && (idx$ < C[Net#e]) ==> (M[Net#e][idx$] == M[Net#c][idx$])
+  );
   assume (1 <= (C[Net#a] - R[Net#a])) && (1 <= (C[Net#b] - R[Net#b]));
+  assume R[Net#a] == C[Net#c];
+  assume R[Net#b] == C[Net#c];
+  assume (forall idx$: int :: 
+    (0 <= idx$) && (idx$ < C[Net#c]) ==> (M[Net#c][idx$] == (M[Net#a][idx$] + M[Net#b][idx$]))
+  );
   in1#i := M[Net#a][R[Net#a]];
   R[Net#a] := R[Net#a] + 1;
   in2#j := M[Net#b][R[Net#b]];
   R[Net#b] := R[Net#b] + 1;
   M[Net#c][C[Net#c]] := in1#i + in2#j;
   C[Net#c] := C[Net#c] + 1;
-  M[Net#d][C[Net#d]] := in1#i + in2#j;
-  C[Net#d] := C[Net#d] + 1;
-  assert {:msg "  Action at 3.3 ('anon$0') for actor instance 'add' might not preserve the channel invariant (#22)"} (forall i: int :: 
-    (0 <= i) && (i < C[Net#a]) ==> (0 < M[Net#a][i])
-  );
-  assert {:msg "  Action at 3.3 ('anon$0') for actor instance 'add' might not preserve the channel invariant (#23)"} R[Net#a] == C[Net#c];
-  assert {:msg "  Action at 3.3 ('anon$0') for actor instance 'add' might not preserve the channel invariant (#24)"} R[Net#b] == C[Net#c];
-  assert {:msg "  Action at 3.3 ('anon$0') for actor instance 'add' might not preserve the channel invariant (#25)"} R[Net#a] == C[Net#d];
-  assert {:msg "  Action at 3.3 ('anon$0') for actor instance 'add' might not preserve the channel invariant (#26)"} R[Net#b] == C[Net#d];
-  assert {:msg "  Action at 3.3 ('anon$0') for actor instance 'add' might not preserve the channel invariant (#27)"} R[Net#d] == (C[Net#b] - 1);
-  assert {:msg "  Action at 3.3 ('anon$0') for actor instance 'add' might not preserve the channel invariant (#28)"} (forall idx$: int :: 
+  assume R[Net#a] == C[Net#c];
+  assume R[Net#b] == C[Net#c];
+  assume (forall idx$: int :: 
     (0 <= idx$) && (idx$ < C[Net#c]) ==> (M[Net#c][idx$] == (M[Net#a][idx$] + M[Net#b][idx$]))
   );
-  assert {:msg "  Action at 3.3 ('anon$0') for actor instance 'add' might not preserve the channel invariant (#29)"} (forall idx$: int :: 
-    (0 <= idx$) && (idx$ < C[Net#d]) ==> (M[Net#d][idx$] == (M[Net#a][idx$] + M[Net#b][idx$]))
+  assert {:msg "25.15: Action at 2.3 ('anon$0') for actor instance 'add' might not preserve the channel invariant (#33)"} (0 < I[Net#d]) ==> (M[Net#d][0] == M[Net#a][0]);
+  assert {:msg "26.15: Action at 2.3 ('anon$0') for actor instance 'add' might not preserve the channel invariant (#34)"} (0 < I[Net#d]) ==> (M[Net#d][I[Net#d] - 1] == M[Net#b][I[Net#b]]);
+  assert {:msg "Action at 2.3 ('anon$0') for actor instance 'add' might not preserve the channel invariant (#35)"} I[Net#c] == I[Net#a];
+  assert {:msg "Action at 2.3 ('anon$0') for actor instance 'add' might not preserve the channel invariant (#36)"} I[Net#c] == I[Net#b];
+  assert {:msg "Action at 2.3 ('anon$0') for actor instance 'add' might not preserve the channel invariant (#37)"} I[Net#b] == I[Net#e];
+  assert {:msg "Action at 2.3 ('anon$0') for actor instance 'add' might not preserve the channel invariant (#38)"} I[Net#d] == I[Net#c];
+  assert {:msg "Action at 2.3 ('anon$0') for actor instance 'add' might not preserve the channel invariant (#39)"} I[Net#e] == I[Net#c];
+  assert {:msg "Action at 2.3 ('anon$0') for actor instance 'add' might not preserve the channel invariant (#40)"} true && (forall idx$: int :: 
+    (I[Net#a] <= idx$) && (idx$ < C[Net#a]) ==> (0 <= M[Net#a][idx$])
   );
-  assert {:msg "  Action at 3.3 ('anon$0') for actor instance 'add' might not preserve the channel invariant (#30)"} (forall idx$: int :: 
-    (1 <= idx$) && (idx$ < C[Net#b]) ==> (M[Net#b][idx$] == M[Net#d][idx$ - 1])
-  );
-  assert {:msg "  22.15: Action at 3.3 ('anon$0') for actor instance 'add' might not preserve the channel invariant (#31)"} I[Net#a] == I[Net#c];
-  assert {:msg "  23.15: Action at 3.3 ('anon$0') for actor instance 'add' might not preserve the channel invariant (#32)"} M[Net#b][0] == 0;
 }
-procedure Net#anon$3#Delay#anon$2#6()
+procedure Net##Delay#anon$3#8()
   modifies C, R, M, I, St;
 {
-  var ActorParam#k: int;
-  var St#next: State;
+  var Net#add: Actor;
+  var Net#del: Actor;
+  var Net#spl: Actor;
+  var Net#a: Chan (int);
+  var Net#b: Chan (int);
+  var Net#c: Chan (int);
+  var Net#d: Chan (int);
+  var Net#e: Chan (int);
   var in#i: int;
+  assume (Net#add != Net#del) && (Net#add != Net#spl) && (Net#del != Net#spl);
+  assume (Net#a != Net#b) && (Net#a != Net#c) && (Net#a != Net#d) && (Net#a != Net#e) && (Net#b != Net#c) && (Net#b != Net#d) && (Net#b != Net#e) && (Net#c != Net#d) && (Net#c != Net#e) && (Net#d != Net#e);
   assume 0 <= I[Net#a];
   assume I[Net#a] <= R[Net#a];
   assume R[Net#a] <= C[Net#a];
@@ -258,61 +355,81 @@ procedure Net#anon$3#Delay#anon$2#6()
   assume 0 <= I[Net#c];
   assume I[Net#c] <= R[Net#c];
   assume R[Net#c] <= C[Net#c];
-  assume I[Net#c] == R[Net#c];
   assume 0 <= I[Net#d];
   assume I[Net#d] <= R[Net#d];
   assume R[Net#d] <= C[Net#d];
-  assume ActorParam#k == 0;
-  assume L[Net#a] == (1 * Base#L);
-  assume (R[Net#a] - I[Net#a]) <= L[Net#a];
-  assume (forall i: int :: 
-    (0 <= i) && (i < C[Net#a]) ==> (0 < M[Net#a][i])
+  assume I[Net#d] == R[Net#d];
+  assume 0 <= I[Net#e];
+  assume I[Net#e] <= R[Net#e];
+  assume R[Net#e] <= C[Net#e];
+  assume (0 < I[Net#d]) ==> (M[Net#d][0] == M[Net#a][0]);
+  assume (0 < I[Net#d]) ==> (M[Net#d][I[Net#d] - 1] == M[Net#b][I[Net#b]]);
+  assume I[Net#c] == I[Net#a];
+  assume I[Net#c] == I[Net#b];
+  assume I[Net#b] == I[Net#e];
+  assume I[Net#d] == I[Net#c];
+  assume I[Net#e] == I[Net#c];
+  assume true && (forall idx$: int :: 
+    (I[Net#a] <= idx$) && (idx$ < C[Net#a]) ==> (0 <= M[Net#a][idx$])
   );
   assume R[Net#a] == C[Net#c];
   assume R[Net#b] == C[Net#c];
-  assume R[Net#a] == C[Net#d];
-  assume R[Net#b] == C[Net#d];
-  assume R[Net#d] == (C[Net#b] - 1);
   assume (forall idx$: int :: 
     (0 <= idx$) && (idx$ < C[Net#c]) ==> (M[Net#c][idx$] == (M[Net#a][idx$] + M[Net#b][idx$]))
   );
-  assume (forall idx$: int :: 
-    (0 <= idx$) && (idx$ < C[Net#d]) ==> (M[Net#d][idx$] == (M[Net#a][idx$] + M[Net#b][idx$]))
-  );
-  assume (forall idx$: int :: 
-    (1 <= idx$) && (idx$ < C[Net#b]) ==> (M[Net#b][idx$] == M[Net#d][idx$ - 1])
-  );
-  assume I[Net#a] == I[Net#c];
   assume M[Net#b][0] == 0;
-  assume true;
-  assume 1 <= (C[Net#d] - R[Net#d]);
-  in#i := M[Net#d][R[Net#d]];
-  R[Net#d] := R[Net#d] + 1;
+  assume R[Net#e] == (C[Net#b] - 1);
+  assume (forall idx$: int :: 
+    (1 <= idx$) && (idx$ < C[Net#b]) ==> (M[Net#b][idx$] == M[Net#e][idx$ - 1])
+  );
+  assume R[Net#c] == C[Net#d];
+  assume R[Net#c] == C[Net#e];
+  assume (forall idx$: int :: 
+    (0 <= idx$) && (idx$ < C[Net#d]) ==> (M[Net#d][idx$] == M[Net#c][idx$])
+  );
+  assume (forall idx$: int :: 
+    (0 <= idx$) && (idx$ < C[Net#e]) ==> (M[Net#e][idx$] == M[Net#c][idx$])
+  );
+  assume 1 <= (C[Net#e] - R[Net#e]);
+  assume M[Net#b][0] == 0;
+  assume R[Net#e] == (C[Net#b] - 1);
+  assume (forall idx$: int :: 
+    (1 <= idx$) && (idx$ < C[Net#b]) ==> (M[Net#b][idx$] == M[Net#e][idx$ - 1])
+  );
+  in#i := M[Net#e][R[Net#e]];
+  R[Net#e] := R[Net#e] + 1;
   M[Net#b][C[Net#b]] := in#i;
   C[Net#b] := C[Net#b] + 1;
-  assert {:msg "  Action at 9.3 ('anon$2') for actor instance 'del' might not preserve the channel invariant (#33)"} (forall i: int :: 
-    (0 <= i) && (i < C[Net#a]) ==> (0 < M[Net#a][i])
+  assume M[Net#b][0] == 0;
+  assume R[Net#e] == (C[Net#b] - 1);
+  assume (forall idx$: int :: 
+    (1 <= idx$) && (idx$ < C[Net#b]) ==> (M[Net#b][idx$] == M[Net#e][idx$ - 1])
   );
-  assert {:msg "  Action at 9.3 ('anon$2') for actor instance 'del' might not preserve the channel invariant (#34)"} R[Net#a] == C[Net#c];
-  assert {:msg "  Action at 9.3 ('anon$2') for actor instance 'del' might not preserve the channel invariant (#35)"} R[Net#b] == C[Net#c];
-  assert {:msg "  Action at 9.3 ('anon$2') for actor instance 'del' might not preserve the channel invariant (#36)"} R[Net#a] == C[Net#d];
-  assert {:msg "  Action at 9.3 ('anon$2') for actor instance 'del' might not preserve the channel invariant (#37)"} R[Net#b] == C[Net#d];
-  assert {:msg "  Action at 9.3 ('anon$2') for actor instance 'del' might not preserve the channel invariant (#38)"} R[Net#d] == (C[Net#b] - 1);
-  assert {:msg "  Action at 9.3 ('anon$2') for actor instance 'del' might not preserve the channel invariant (#39)"} (forall idx$: int :: 
-    (0 <= idx$) && (idx$ < C[Net#c]) ==> (M[Net#c][idx$] == (M[Net#a][idx$] + M[Net#b][idx$]))
+  assert {:msg "25.15: Action at 12.3 ('anon$3') for actor instance 'del' might not preserve the channel invariant (#41)"} (0 < I[Net#d]) ==> (M[Net#d][0] == M[Net#a][0]);
+  assert {:msg "26.15: Action at 12.3 ('anon$3') for actor instance 'del' might not preserve the channel invariant (#42)"} (0 < I[Net#d]) ==> (M[Net#d][I[Net#d] - 1] == M[Net#b][I[Net#b]]);
+  assert {:msg "Action at 12.3 ('anon$3') for actor instance 'del' might not preserve the channel invariant (#43)"} I[Net#c] == I[Net#a];
+  assert {:msg "Action at 12.3 ('anon$3') for actor instance 'del' might not preserve the channel invariant (#44)"} I[Net#c] == I[Net#b];
+  assert {:msg "Action at 12.3 ('anon$3') for actor instance 'del' might not preserve the channel invariant (#45)"} I[Net#b] == I[Net#e];
+  assert {:msg "Action at 12.3 ('anon$3') for actor instance 'del' might not preserve the channel invariant (#46)"} I[Net#d] == I[Net#c];
+  assert {:msg "Action at 12.3 ('anon$3') for actor instance 'del' might not preserve the channel invariant (#47)"} I[Net#e] == I[Net#c];
+  assert {:msg "Action at 12.3 ('anon$3') for actor instance 'del' might not preserve the channel invariant (#48)"} true && (forall idx$: int :: 
+    (I[Net#a] <= idx$) && (idx$ < C[Net#a]) ==> (0 <= M[Net#a][idx$])
   );
-  assert {:msg "  Action at 9.3 ('anon$2') for actor instance 'del' might not preserve the channel invariant (#40)"} (forall idx$: int :: 
-    (0 <= idx$) && (idx$ < C[Net#d]) ==> (M[Net#d][idx$] == (M[Net#a][idx$] + M[Net#b][idx$]))
-  );
-  assert {:msg "  Action at 9.3 ('anon$2') for actor instance 'del' might not preserve the channel invariant (#41)"} (forall idx$: int :: 
-    (1 <= idx$) && (idx$ < C[Net#b]) ==> (M[Net#b][idx$] == M[Net#d][idx$ - 1])
-  );
-  assert {:msg "  22.15: Action at 9.3 ('anon$2') for actor instance 'del' might not preserve the channel invariant (#42)"} I[Net#a] == I[Net#c];
-  assert {:msg "  23.15: Action at 9.3 ('anon$2') for actor instance 'del' might not preserve the channel invariant (#43)"} M[Net#b][0] == 0;
 }
-procedure Net#anon$3#exit#7()
+procedure Net##Split#anon$1#9()
   modifies C, R, M, I, St;
 {
+  var Net#add: Actor;
+  var Net#del: Actor;
+  var Net#spl: Actor;
+  var Net#a: Chan (int);
+  var Net#b: Chan (int);
+  var Net#c: Chan (int);
+  var Net#d: Chan (int);
+  var Net#e: Chan (int);
+  var in#i: int;
+  assume (Net#add != Net#del) && (Net#add != Net#spl) && (Net#del != Net#spl);
+  assume (Net#a != Net#b) && (Net#a != Net#c) && (Net#a != Net#d) && (Net#a != Net#e) && (Net#b != Net#c) && (Net#b != Net#d) && (Net#b != Net#e) && (Net#c != Net#d) && (Net#c != Net#e) && (Net#d != Net#e);
   assume 0 <= I[Net#a];
   assume I[Net#a] <= R[Net#a];
   assume R[Net#a] <= C[Net#a];
@@ -322,62 +439,293 @@ procedure Net#anon$3#exit#7()
   assume 0 <= I[Net#c];
   assume I[Net#c] <= R[Net#c];
   assume R[Net#c] <= C[Net#c];
-  assume I[Net#c] == R[Net#c];
   assume 0 <= I[Net#d];
   assume I[Net#d] <= R[Net#d];
   assume R[Net#d] <= C[Net#d];
-  assume L[Net#a] == (1 * Base#L);
-  assume (R[Net#a] - I[Net#a]) <= L[Net#a];
-  assume (forall i: int :: 
-    (0 <= i) && (i < C[Net#a]) ==> (0 < M[Net#a][i])
+  assume I[Net#d] == R[Net#d];
+  assume 0 <= I[Net#e];
+  assume I[Net#e] <= R[Net#e];
+  assume R[Net#e] <= C[Net#e];
+  assume (0 < I[Net#d]) ==> (M[Net#d][0] == M[Net#a][0]);
+  assume (0 < I[Net#d]) ==> (M[Net#d][I[Net#d] - 1] == M[Net#b][I[Net#b]]);
+  assume I[Net#c] == I[Net#a];
+  assume I[Net#c] == I[Net#b];
+  assume I[Net#b] == I[Net#e];
+  assume I[Net#d] == I[Net#c];
+  assume I[Net#e] == I[Net#c];
+  assume true && (forall idx$: int :: 
+    (I[Net#a] <= idx$) && (idx$ < C[Net#a]) ==> (0 <= M[Net#a][idx$])
   );
   assume R[Net#a] == C[Net#c];
   assume R[Net#b] == C[Net#c];
-  assume R[Net#a] == C[Net#d];
-  assume R[Net#b] == C[Net#d];
-  assume R[Net#d] == (C[Net#b] - 1);
   assume (forall idx$: int :: 
     (0 <= idx$) && (idx$ < C[Net#c]) ==> (M[Net#c][idx$] == (M[Net#a][idx$] + M[Net#b][idx$]))
   );
-  assume (forall idx$: int :: 
-    (0 <= idx$) && (idx$ < C[Net#d]) ==> (M[Net#d][idx$] == (M[Net#a][idx$] + M[Net#b][idx$]))
-  );
-  assume (forall idx$: int :: 
-    (1 <= idx$) && (idx$ < C[Net#b]) ==> (M[Net#b][idx$] == M[Net#d][idx$ - 1])
-  );
-  assume I[Net#a] == I[Net#c];
   assume M[Net#b][0] == 0;
-  assume !((R[Net#a] - I[Net#a]) < L[Net#a]);
-  assume !((1 <= (C[Net#a] - R[Net#a])) && (1 <= (C[Net#b] - R[Net#b])));
-  assume !(1 <= (C[Net#d] - R[Net#d]));
-  assert {:msg "  16.13: Network action postcondition might not hold"} M[Net#c][0] == M[Net#a][0];
-  assert {:msg "  17.14: Network action postcondition might not hold"} (forall i: int :: 
-    (1 <= i) && (i < C[Net#c]) ==> (M[Net#c][i] == (M[Net#a][i] + M[Net#c][i - 1]))
+  assume R[Net#e] == (C[Net#b] - 1);
+  assume (forall idx$: int :: 
+    (1 <= idx$) && (idx$ < C[Net#b]) ==> (M[Net#b][idx$] == M[Net#e][idx$ - 1])
   );
-  R[Net#c] := R[Net#c] + (1 * Base#L);
-  I := R;
-  assert {:msg "  The network might not preserve the channel invariant (#44)"} (forall i: int :: 
-    (0 <= i) && (i < C[Net#a]) ==> (0 < M[Net#a][i])
+  assume R[Net#c] == C[Net#d];
+  assume R[Net#c] == C[Net#e];
+  assume (forall idx$: int :: 
+    (0 <= idx$) && (idx$ < C[Net#d]) ==> (M[Net#d][idx$] == M[Net#c][idx$])
   );
-  assert {:msg "  The network might not preserve the channel invariant (#45)"} R[Net#a] == C[Net#c];
-  assert {:msg "  The network might not preserve the channel invariant (#46)"} R[Net#b] == C[Net#c];
-  assert {:msg "  The network might not preserve the channel invariant (#47)"} R[Net#a] == C[Net#d];
-  assert {:msg "  The network might not preserve the channel invariant (#48)"} R[Net#b] == C[Net#d];
-  assert {:msg "  The network might not preserve the channel invariant (#49)"} R[Net#d] == (C[Net#b] - 1);
-  assert {:msg "  The network might not preserve the channel invariant (#50)"} (forall idx$: int :: 
+  assume (forall idx$: int :: 
+    (0 <= idx$) && (idx$ < C[Net#e]) ==> (M[Net#e][idx$] == M[Net#c][idx$])
+  );
+  assume 1 <= (C[Net#c] - R[Net#c]);
+  assume R[Net#c] == C[Net#d];
+  assume R[Net#c] == C[Net#e];
+  assume (forall idx$: int :: 
+    (0 <= idx$) && (idx$ < C[Net#d]) ==> (M[Net#d][idx$] == M[Net#c][idx$])
+  );
+  assume (forall idx$: int :: 
+    (0 <= idx$) && (idx$ < C[Net#e]) ==> (M[Net#e][idx$] == M[Net#c][idx$])
+  );
+  in#i := M[Net#c][R[Net#c]];
+  R[Net#c] := R[Net#c] + 1;
+  M[Net#d][C[Net#d]] := in#i;
+  C[Net#d] := C[Net#d] + 1;
+  M[Net#e][C[Net#e]] := in#i;
+  C[Net#e] := C[Net#e] + 1;
+  assume R[Net#c] == C[Net#d];
+  assume R[Net#c] == C[Net#e];
+  assume (forall idx$: int :: 
+    (0 <= idx$) && (idx$ < C[Net#d]) ==> (M[Net#d][idx$] == M[Net#c][idx$])
+  );
+  assume (forall idx$: int :: 
+    (0 <= idx$) && (idx$ < C[Net#e]) ==> (M[Net#e][idx$] == M[Net#c][idx$])
+  );
+  assert {:msg "25.15: Action at 6.3 ('anon$1') for actor instance 'spl' might not preserve the channel invariant (#49)"} (0 < I[Net#d]) ==> (M[Net#d][0] == M[Net#a][0]);
+  assert {:msg "26.15: Action at 6.3 ('anon$1') for actor instance 'spl' might not preserve the channel invariant (#50)"} (0 < I[Net#d]) ==> (M[Net#d][I[Net#d] - 1] == M[Net#b][I[Net#b]]);
+  assert {:msg "Action at 6.3 ('anon$1') for actor instance 'spl' might not preserve the channel invariant (#51)"} I[Net#c] == I[Net#a];
+  assert {:msg "Action at 6.3 ('anon$1') for actor instance 'spl' might not preserve the channel invariant (#52)"} I[Net#c] == I[Net#b];
+  assert {:msg "Action at 6.3 ('anon$1') for actor instance 'spl' might not preserve the channel invariant (#53)"} I[Net#b] == I[Net#e];
+  assert {:msg "Action at 6.3 ('anon$1') for actor instance 'spl' might not preserve the channel invariant (#54)"} I[Net#d] == I[Net#c];
+  assert {:msg "Action at 6.3 ('anon$1') for actor instance 'spl' might not preserve the channel invariant (#55)"} I[Net#e] == I[Net#c];
+  assert {:msg "Action at 6.3 ('anon$1') for actor instance 'spl' might not preserve the channel invariant (#56)"} true && (forall idx$: int :: 
+    (I[Net#a] <= idx$) && (idx$ < C[Net#a]) ==> (0 <= M[Net#a][idx$])
+  );
+}
+procedure Net#entry()
+  modifies C, R, M, I, St;
+{
+  var Net#add: Actor;
+  var Net#del: Actor;
+  var Net#spl: Actor;
+  var Net#a: Chan (int);
+  var Net#b: Chan (int);
+  var Net#c: Chan (int);
+  var Net#d: Chan (int);
+  var Net#e: Chan (int);
+  assume (Net#add != Net#del) && (Net#add != Net#spl) && (Net#del != Net#spl);
+  assume (Net#a != Net#b) && (Net#a != Net#c) && (Net#a != Net#d) && (Net#a != Net#e) && (Net#b != Net#c) && (Net#b != Net#d) && (Net#b != Net#e) && (Net#c != Net#d) && (Net#c != Net#e) && (Net#d != Net#e);
+  assume 0 <= I[Net#a];
+  assume I[Net#a] <= R[Net#a];
+  assume R[Net#a] <= C[Net#a];
+  assume 0 <= I[Net#b];
+  assume I[Net#b] <= R[Net#b];
+  assume R[Net#b] <= C[Net#b];
+  assume 0 <= I[Net#c];
+  assume I[Net#c] <= R[Net#c];
+  assume R[Net#c] <= C[Net#c];
+  assume 0 <= I[Net#d];
+  assume I[Net#d] <= R[Net#d];
+  assume R[Net#d] <= C[Net#d];
+  assume I[Net#d] == R[Net#d];
+  assume 0 <= I[Net#e];
+  assume I[Net#e] <= R[Net#e];
+  assume R[Net#e] <= C[Net#e];
+  assume C[Net#a] == R[Net#a];
+  assume C[Net#b] == R[Net#b];
+  assume C[Net#c] == R[Net#c];
+  assume C[Net#d] == R[Net#d];
+  assume C[Net#e] == R[Net#e];
+  C[Net#b] := C[Net#b] + 1;
+  assume (0 < I[Net#d]) ==> (M[Net#d][0] == M[Net#a][0]);
+  assume (0 < I[Net#d]) ==> (M[Net#d][I[Net#d] - 1] == M[Net#b][I[Net#b]]);
+  assume I[Net#c] == I[Net#a];
+  assume I[Net#c] == I[Net#b];
+  assume I[Net#b] == I[Net#e];
+  assume I[Net#d] == I[Net#c];
+  assume I[Net#e] == I[Net#c];
+  assume true && (forall idx$: int :: 
+    (I[Net#a] <= idx$) && (idx$ < C[Net#a]) ==> (0 <= M[Net#a][idx$])
+  );
+  assume R[Net#a] == C[Net#c];
+  assume R[Net#b] == C[Net#c];
+  assume (forall idx$: int :: 
     (0 <= idx$) && (idx$ < C[Net#c]) ==> (M[Net#c][idx$] == (M[Net#a][idx$] + M[Net#b][idx$]))
   );
-  assert {:msg "  The network might not preserve the channel invariant (#51)"} (forall idx$: int :: 
-    (0 <= idx$) && (idx$ < C[Net#d]) ==> (M[Net#d][idx$] == (M[Net#a][idx$] + M[Net#b][idx$]))
+  assume M[Net#b][0] == 0;
+  assume R[Net#e] == (C[Net#b] - 1);
+  assume (forall idx$: int :: 
+    (1 <= idx$) && (idx$ < C[Net#b]) ==> (M[Net#b][idx$] == M[Net#e][idx$ - 1])
   );
-  assert {:msg "  The network might not preserve the channel invariant (#52)"} (forall idx$: int :: 
-    (1 <= idx$) && (idx$ < C[Net#b]) ==> (M[Net#b][idx$] == M[Net#d][idx$ - 1])
+  assume R[Net#c] == C[Net#d];
+  assume R[Net#c] == C[Net#e];
+  assume (forall idx$: int :: 
+    (0 <= idx$) && (idx$ < C[Net#d]) ==> (M[Net#d][idx$] == M[Net#c][idx$])
   );
-  assert {:msg "  22.15: The network might not preserve the channel invariant (#53)"} I[Net#a] == I[Net#c];
-  assert {:msg "  23.15: The network might not preserve the channel invariant (#54)"} M[Net#b][0] == 0;
+  assume (forall idx$: int :: 
+    (0 <= idx$) && (idx$ < C[Net#e]) ==> (M[Net#e][idx$] == M[Net#c][idx$])
+  );
+  assert {:msg "15.1: Sub-actors in the network might fire without network input. This is not permitted. (#57)"} !((1 <= (C[Net#a] - R[Net#a])) && (1 <= (C[Net#b] - R[Net#b])));
+  assert {:msg "15.1: Sub-actors in the network might fire without network input. This is not permitted. (#58)"} !(1 <= (C[Net#e] - R[Net#e]));
+  assert {:msg "15.1: Sub-actors in the network might fire without network input. This is not permitted. (#59)"} !(1 <= (C[Net#c] - R[Net#c]));
+}
+procedure Net#anon$4#input#in#10()
+  modifies C, R, M, I, St;
+{
+  var Net#add: Actor;
+  var Net#del: Actor;
+  var Net#spl: Actor;
+  var Net#a: Chan (int);
+  var Net#b: Chan (int);
+  var Net#c: Chan (int);
+  var Net#d: Chan (int);
+  var Net#e: Chan (int);
+  assume (Net#add != Net#del) && (Net#add != Net#spl) && (Net#del != Net#spl);
+  assume (Net#a != Net#b) && (Net#a != Net#c) && (Net#a != Net#d) && (Net#a != Net#e) && (Net#b != Net#c) && (Net#b != Net#d) && (Net#b != Net#e) && (Net#c != Net#d) && (Net#c != Net#e) && (Net#d != Net#e);
+  assume 0 <= I[Net#a];
+  assume I[Net#a] <= R[Net#a];
+  assume R[Net#a] <= C[Net#a];
+  assume 0 <= I[Net#b];
+  assume I[Net#b] <= R[Net#b];
+  assume R[Net#b] <= C[Net#b];
+  assume 0 <= I[Net#c];
+  assume I[Net#c] <= R[Net#c];
+  assume R[Net#c] <= C[Net#c];
+  assume 0 <= I[Net#d];
+  assume I[Net#d] <= R[Net#d];
+  assume R[Net#d] <= C[Net#d];
+  assume I[Net#d] == R[Net#d];
+  assume 0 <= I[Net#e];
+  assume I[Net#e] <= R[Net#e];
+  assume R[Net#e] <= C[Net#e];
+  assume C[Net#a] < 1;
+  assume (0 < I[Net#d]) ==> (M[Net#d][0] == M[Net#a][0]);
+  assume (0 < I[Net#d]) ==> (M[Net#d][I[Net#d] - 1] == M[Net#b][I[Net#b]]);
+  assume I[Net#c] == I[Net#a];
+  assume I[Net#c] == I[Net#b];
+  assume I[Net#b] == I[Net#e];
+  assume I[Net#d] == I[Net#c];
+  assume I[Net#e] == I[Net#c];
+  assume true && (forall idx$: int :: 
+    (I[Net#a] <= idx$) && (idx$ < C[Net#a]) ==> (0 <= M[Net#a][idx$])
+  );
+  assume R[Net#a] == C[Net#c];
+  assume R[Net#b] == C[Net#c];
+  assume (forall idx$: int :: 
+    (0 <= idx$) && (idx$ < C[Net#c]) ==> (M[Net#c][idx$] == (M[Net#a][idx$] + M[Net#b][idx$]))
+  );
+  assume M[Net#b][0] == 0;
+  assume R[Net#e] == (C[Net#b] - 1);
+  assume (forall idx$: int :: 
+    (1 <= idx$) && (idx$ < C[Net#b]) ==> (M[Net#b][idx$] == M[Net#e][idx$ - 1])
+  );
+  assume R[Net#c] == C[Net#d];
+  assume R[Net#c] == C[Net#e];
+  assume (forall idx$: int :: 
+    (0 <= idx$) && (idx$ < C[Net#d]) ==> (M[Net#d][idx$] == M[Net#c][idx$])
+  );
+  assume (forall idx$: int :: 
+    (0 <= idx$) && (idx$ < C[Net#e]) ==> (M[Net#e][idx$] == M[Net#c][idx$])
+  );
+  C[Net#a] := C[Net#a] + 1;
+  assume 0 <= M[Net#a][I[Net#a]];
+  assert {:msg "25.15: Channel invariant might be falsified by network input (#60)"} (0 < I[Net#d]) ==> (M[Net#d][0] == M[Net#a][0]);
+  assert {:msg "26.15: Channel invariant might be falsified by network input (#61)"} (0 < I[Net#d]) ==> (M[Net#d][I[Net#d] - 1] == M[Net#b][I[Net#b]]);
+  assert {:msg "Channel invariant might be falsified by network input (#62)"} I[Net#c] == I[Net#a];
+  assert {:msg "Channel invariant might be falsified by network input (#63)"} I[Net#c] == I[Net#b];
+  assert {:msg "Channel invariant might be falsified by network input (#64)"} I[Net#b] == I[Net#e];
+  assert {:msg "Channel invariant might be falsified by network input (#65)"} I[Net#d] == I[Net#c];
+  assert {:msg "Channel invariant might be falsified by network input (#66)"} I[Net#e] == I[Net#c];
+  assert {:msg "Channel invariant might be falsified by network input (#67)"} true && (forall idx$: int :: 
+    (I[Net#a] <= idx$) && (idx$ < C[Net#a]) ==> (0 <= M[Net#a][idx$])
+  );
+}
+procedure Net#anon$4#exit#11()
+  modifies C, R, M, I, St;
+{
+  var Net#add: Actor;
+  var Net#del: Actor;
+  var Net#spl: Actor;
+  var Net#a: Chan (int);
+  var Net#b: Chan (int);
+  var Net#c: Chan (int);
+  var Net#d: Chan (int);
+  var Net#e: Chan (int);
+  assume (Net#add != Net#del) && (Net#add != Net#spl) && (Net#del != Net#spl);
+  assume (Net#a != Net#b) && (Net#a != Net#c) && (Net#a != Net#d) && (Net#a != Net#e) && (Net#b != Net#c) && (Net#b != Net#d) && (Net#b != Net#e) && (Net#c != Net#d) && (Net#c != Net#e) && (Net#d != Net#e);
+  assume 0 <= I[Net#a];
+  assume I[Net#a] <= R[Net#a];
+  assume R[Net#a] <= C[Net#a];
+  assume 0 <= I[Net#b];
+  assume I[Net#b] <= R[Net#b];
+  assume R[Net#b] <= C[Net#b];
+  assume 0 <= I[Net#c];
+  assume I[Net#c] <= R[Net#c];
+  assume R[Net#c] <= C[Net#c];
+  assume 0 <= I[Net#d];
+  assume I[Net#d] <= R[Net#d];
+  assume R[Net#d] <= C[Net#d];
+  assume I[Net#d] == R[Net#d];
+  assume 0 <= I[Net#e];
+  assume I[Net#e] <= R[Net#e];
+  assume R[Net#e] <= C[Net#e];
+  assume (0 < I[Net#d]) ==> (M[Net#d][0] == M[Net#a][0]);
+  assume (0 < I[Net#d]) ==> (M[Net#d][I[Net#d] - 1] == M[Net#b][I[Net#b]]);
+  assume I[Net#c] == I[Net#a];
+  assume I[Net#c] == I[Net#b];
+  assume I[Net#b] == I[Net#e];
+  assume I[Net#d] == I[Net#c];
+  assume I[Net#e] == I[Net#c];
+  assume true && (forall idx$: int :: 
+    (I[Net#a] <= idx$) && (idx$ < C[Net#a]) ==> (0 <= M[Net#a][idx$])
+  );
+  assume R[Net#a] == C[Net#c];
+  assume R[Net#b] == C[Net#c];
+  assume (forall idx$: int :: 
+    (0 <= idx$) && (idx$ < C[Net#c]) ==> (M[Net#c][idx$] == (M[Net#a][idx$] + M[Net#b][idx$]))
+  );
+  assume M[Net#b][0] == 0;
+  assume R[Net#e] == (C[Net#b] - 1);
+  assume (forall idx$: int :: 
+    (1 <= idx$) && (idx$ < C[Net#b]) ==> (M[Net#b][idx$] == M[Net#e][idx$ - 1])
+  );
+  assume R[Net#c] == C[Net#d];
+  assume R[Net#c] == C[Net#e];
+  assume (forall idx$: int :: 
+    (0 <= idx$) && (idx$ < C[Net#d]) ==> (M[Net#d][idx$] == M[Net#c][idx$])
+  );
+  assume (forall idx$: int :: 
+    (0 <= idx$) && (idx$ < C[Net#e]) ==> (M[Net#e][idx$] == M[Net#c][idx$])
+  );
+  assume (C[Net#a] - I[Net#a]) == 1;
+  assume 0 <= M[Net#a][I[Net#a]];
+  assume !((1 <= (C[Net#a] - R[Net#a])) && (1 <= (C[Net#b] - R[Net#b])));
+  assume !(1 <= (C[Net#e] - R[Net#e]));
+  assume !(1 <= (C[Net#c] - R[Net#c]));
+  assert {:msg "19.13: Network action postcondition might not hold (#68)"} M[Net#d][0] == M[Net#a][0];
+  assert {:msg "20.13: Network action postcondition might not hold (#69)"} (0 < I[Net#d]) ==> (M[Net#d][I[Net#d]] == (M[Net#d][I[Net#d] - 1] + M[Net#a][I[Net#a]]));
+  R[Net#d] := R[Net#d] + 1;
+  I := R;
+  assert {:msg "25.15: The network might not preserve the channel invariant (#70)"} (0 < I[Net#d]) ==> (M[Net#d][0] == M[Net#a][0]);
+  assert {:msg "26.15: The network might not preserve the channel invariant (#71)"} (0 < I[Net#d]) ==> (M[Net#d][I[Net#d] - 1] == M[Net#b][I[Net#b]]);
+  assert {:msg "The network might not preserve the channel invariant (#72)"} I[Net#c] == I[Net#a];
+  assert {:msg "The network might not preserve the channel invariant (#73)"} I[Net#c] == I[Net#b];
+  assert {:msg "The network might not preserve the channel invariant (#74)"} I[Net#b] == I[Net#e];
+  assert {:msg "The network might not preserve the channel invariant (#75)"} I[Net#d] == I[Net#c];
+  assert {:msg "The network might not preserve the channel invariant (#76)"} I[Net#e] == I[Net#c];
+  assert {:msg "The network might not preserve the channel invariant (#77)"} true && (forall idx$: int :: 
+    (I[Net#a] <= idx$) && (idx$ < C[Net#a]) ==> (0 <= M[Net#a][idx$])
+  );
   C[Net#b] := C[Net#b] - 1;
-  assert {:msg "  14.3: The network might leave unread tokens on channel a"} (C[Net#a] - R[Net#a]) == 0;
-  assert {:msg "  14.3: The network might leave unread tokens on channel b"} (C[Net#b] - R[Net#b]) == 0;
-  assert {:msg "  14.3: The network might not produce the specified number of tokens on output out"} (C[Net#c] - R[Net#c]) == 0;
-  assert {:msg "  14.3: The network might leave unread tokens on channel d"} (C[Net#d] - R[Net#d]) == 0;
+  assert {:msg "17.3: The network might leave unread tokens on channel a (#78)"} C[Net#a] == R[Net#a];
+  assert {:msg "17.3: The network might leave unread tokens on channel b (#79)"} C[Net#b] == R[Net#b];
+  assert {:msg "17.3: The network might leave unread tokens on channel c (#80)"} C[Net#c] == R[Net#c];
+  assert {:msg "17.3: The network might not produce the specified number of tokens on output out (#81)"} C[Net#d] == R[Net#d];
+  assert {:msg "17.3: The network might leave unread tokens on channel e (#82)"} C[Net#e] == R[Net#e];
 }
